clique example, refactor some code

examples/pseudo_bool/array/cliqueProgScript.sml
@@ -1,107 +1,41 @@
 (*
-  MCIS (connected) encode and checker
+  Clique encode and checker
 *)
-open preamble basis pbc_normaliseTheory graphProgTheory mcisTheory graph_basicTheory;
+open preamble basis pbc_normaliseTheory graphProgTheory cliqueTheory graph_basicTheory;
 
-val _ = new_theory "mccisProg"
+val _ = new_theory "cliqueProg"
 
 val _ = translation_extends"graphProg";
 
 val xlet_autop = xlet_auto >- (TRY( xcon) >> xsimpl)
 
 (* The encoder *)
-val _ = translate has_mapping_def;
-val _ = translate all_has_mapping_def;
-val _ = translate one_one_def;
-val _ = translate all_one_one_def;
-
-val _ = translate edge_map_def;
-
-val _ = translate not_edge_map_def;
-val _ = translate all_full_edge_map_def;
-
-val _ = translate encode_base_def;
-
-val _ = translate pbcTheory.negate_def;
-val _ = translate iff_and_def;
-val _ = translate iff_or_def;
-val _ = translate walk_base_def;
-val _ = translate walk_aux_def;
-val _ = translate walk_ind_def;
-val _ = translate walk_k_def;
-
-(* TODO: use PRECONDITION *)
-Definition log2_def:
-  log2 n =
-  if n < 2 then 0:num
-  else (log2 (n DIV 2))+1
-End
-
-Theorem LOG2_log2:
-  ∀n.
-  n ≥ 1 ⇒
-  LOG 2 n = log2 n
-Proof
-  ho_match_mp_tac log2_ind>>rw[]>>
-  simp[Once log2_def]>>rw[]
-  >- (
-    `n=1`by fs[]>>
-    rw[])>>
-  REWRITE_TAC[Once numeral_bitTheory.LOG_compute]>>
-  fs[ADD1]>>
-  first_x_assum match_mp_tac>>
-  intLib.ARITH_TAC
-QED
-
-Theorem encode_connected_thm:
-  encode_connected (vp,ep) =
-  if vp = 0 then []
-  else
-  let k = log2 (vp*2-1) in
-  walk_k (vp,ep) k ++
-  FLAT (GENLIST (λf.
-    FLAT (GENLIST (λg.
-      if f < g then
-        [(GreaterEqual, [(1, Pos(Unmapped f));(1, Pos(Unmapped g));(1, Pos(Walk f g k))], 1)]
-      else []) vp)) vp)
-Proof
-  rw[encode_connected_def]>>
-  DEP_REWRITE_TAC [LOG2_log2]>>
-  fs[]
-QED
-
-val _ = translate log2_def;
-val _ = translate (encode_connected_thm);
+val _ = translate mk_constraint_def;
 val _ = translate encode_def;
 
-(* Translate the string converter *)
+(* The string converter *)
 val res = translate enc_string_def;
 
 val _ = translate pbcTheory.map_obj_def;
-val _ = translate unmapped_obj_def;
+val _ = translate clique_obj_def;
 
-val _ = translate full_encode_mccis_def;
+val _ = translate full_encode_def;
 
-(* parse input from f1 f2 and run encoder into pbc *)
+(* parse input from f and run encoder into pbc *)
 val parse_and_enc = (append_prog o process_topdecs) `
-  fun parse_and_enc f1 f2 =
-  case parse_lad f1 of
+  fun parse_and_enc f =
+  case parse_dimacs f of
     Inl err => Inl err
-  | Inr gp =>
-  (case parse_lad f2 of
-    Inl err => Inl err
-  | Inr gt =>
-    Inr (fst gp, full_encode_mccis gp gt))`
+  | Inr g =>
+    Inr (fst g, full_encode g)`
 
 Theorem parse_and_enc_spec:
-  STRING_TYPE f1 f1v ∧
-  STRING_TYPE f2 f2v ∧
-  validArg f1 ∧
-  validArg f2 ∧
+  STRING_TYPE f fv ∧
+  validArg f ∧
   hasFreeFD fs
   ⇒
   app (p:'ffi ffi_proj) ^(fetch_v"parse_and_enc"(get_ml_prog_state()))
-    [f1v;f2v]
+    [fv]
     (STDIO fs)
     (POSTv v.
     STDIO fs *
@@ -115,14 +49,12 @@ Theorem parse_and_enc_spec:
             )) res v ∧
        case res of
         INL err =>
-          get_graph_lad fs f1 = NONE ∨
-          get_graph_lad fs f2 = NONE
+          get_graph_dimacs fs f = NONE
       | INR (n,objf) =>
-        ∃gp gt.
-        get_graph_lad fs f1 = SOME gp ∧
-        get_graph_lad fs f2 = SOME gt ∧
-        full_encode_mccis gp gt = objf ∧
-        FST gp = n)
+        ∃g.
+          get_graph_dimacs fs f = SOME g ∧
+          full_encode g = objf ∧
+          FST g = n)
 Proof
   rw[]>>
   xcf"parse_and_enc"(get_ml_prog_state())>>
@@ -131,15 +63,10 @@ Proof
   >- (
     xcon>>xsimpl>>
     qexists_tac`INL err`>>simp[SUM_TYPE_def])>>
-  xlet_autop>>
-  every_case_tac>>fs[SUM_TYPE_def]>>xmatch
-  >- (
-    xcon>>xsimpl>>
-    qexists_tac`INL err`>>simp[SUM_TYPE_def])>>
   rpt xlet_autop>>
   xcon>>xsimpl >>
-  rename1`_ (full_encode_mccis gpp gtt)`>>
-  qexists_tac`INR (FST gpp,full_encode_mccis gpp gtt)`>>
+  rename1`_ (full_encode g)`>>
+  qexists_tac`INR (FST g,full_encode g)`>>
   simp[SUM_TYPE_def,PAIR_TYPE_def]
 QED
 
@@ -150,45 +77,43 @@ Definition int_inf_to_string_def:
     toString i)
 End
 
-Definition print_mccis_bound_def:
-  print_mccis_bound (lbg:num option,ubg:num) =
+Definition print_clique_bound_def:
+  print_clique_bound (lbg:num option,ubg:num) =
   case lbg of
     NONE =>
-    strlit "s VERIFIED MCIS BOUNDS " ^ strlit "|MCIS| <= " ^ toString ubg ^ strlit"\n"
+    strlit "s VERIFIED MAX CLIQUE BOUNDS " ^ strlit "|CLIQUE| <= " ^ toString ubg ^ strlit"\n"
   | SOME l =>
-    strlit "s VERIFIED MCIS BOUNDS " ^ toString l ^ strlit " <= |MCIS| <= " ^ toString ubg ^ strlit"\n"
+    strlit "s VERIFIED MAX CLIQUE BOUNDS " ^ toString l ^ strlit " <= |CLIQUE| <= " ^ toString ubg ^ strlit"\n"
 End
 
-Definition mccis_sem_def:
-  mccis_sem gp gt (lbg,ubg) ⇔
-  (∀f vs.
-    injective_partial_map f vs gp gt ∧
-    connected_subgraph vs (SND gp) ⇒
+Definition clique_sem_def:
+  clique_sem g (lbg,ubg) ⇔
+  (∀vs.
+    is_clique vs g ⇒
     CARD vs ≤ ubg) ∧
-  case lbg of NONE => T
+  case lbg of
+    NONE => T
   | SOME lb =>
-    ∃f vs.
-      injective_partial_map f vs gp gt ∧
-      connected_subgraph vs (SND gp) ∧
+    ∃vs.
+      is_clique vs g ∧
       lb ≤ CARD vs
 End
 
-Definition check_unsat_3_sem_def:
-  check_unsat_3_sem fs f1 f2 out ⇔
+Definition check_unsat_2_sem_def:
+  check_unsat_2_sem fs f out ⇔
   (out ≠ strlit"" ⇒
-  ∃gp gt bounds.
-    get_graph_lad fs f1 = SOME gp ∧
-    get_graph_lad fs f2 = SOME gt ∧
-    out = print_mccis_bound bounds ∧
-    mccis_sem gp gt bounds)
+  ∃g bounds.
+    get_graph_dimacs fs f = SOME g ∧
+    out = print_clique_bound bounds ∧
+    clique_sem g bounds)
 End
 
 Definition map_concl_to_string_def:
   (map_concl_to_string n (INL s) = (INL s)) ∧
   (map_concl_to_string n (INR c) =
     case conv_concl n c of
-      SOME bounds => INR (print_mccis_bound bounds)
-    | NONE => INL (strlit "c Unexpected conclusion for MCIS problem.\n"))
+      SOME bounds => INR (print_clique_bound bounds)
+    | NONE => INL (strlit "c Unexpected conclusion for max clique problem.\n"))
 End
 
 val res = translate conv_concl_def;
@@ -199,49 +124,38 @@ val conv_concl_side = Q.prove(
   rw[]>>
   intLib.ARITH_TAC) |> update_precondition;
 
-val res = translate print_mccis_bound_def;
+val res = translate print_clique_bound_def;
 val res = translate map_concl_to_string_def;
 
-val check_unsat_3 = (append_prog o process_topdecs) `
-  fun check_unsat_3 f1 f2 f3 =
-  case parse_and_enc f1 f2 of
+val check_unsat_2 = (append_prog o process_topdecs) `
+  fun check_unsat_2 f1 f2 =
+  case parse_and_enc f1 of
     Inl err => TextIO.output TextIO.stdErr err
   | Inr (n,objf) =>
     (case
       map_concl_to_string n
-        (check_unsat_top_norm objf f3) of
+        (check_unsat_top_norm objf f2) of
       Inl err => TextIO.output TextIO.stdErr err
     | Inr s => TextIO.print s)`
 
-Theorem check_unsat_3_spec:
+Theorem check_unsat_2_spec:
   STRING_TYPE f1 f1v ∧ validArg f1 ∧
   STRING_TYPE f2 f2v ∧ validArg f2 ∧
-  STRING_TYPE f3 f3v ∧ validArg f3 ∧
   hasFreeFD fs
   ⇒
-  app (p:'ffi ffi_proj) ^(fetch_v"check_unsat_3"(get_ml_prog_state()))
-    [f1v; f2v; f3v]
+  app (p:'ffi ffi_proj) ^(fetch_v"check_unsat_2"(get_ml_prog_state()))
+    [f1v; f2v]
     (STDIO fs)
     (POSTv uv. &UNIT_TYPE () uv *
     SEP_EXISTS out err.
       STDIO (add_stdout (add_stderr fs err) out) *
-      &(check_unsat_3_sem fs f1 f2 out))
+      &(check_unsat_2_sem fs f1 out))
 Proof
-  rw[check_unsat_3_sem_def]>>
-  xcf "check_unsat_3" (get_ml_prog_state ())>>
+  rw[check_unsat_2_sem_def]>>
+  xcf "check_unsat_2" (get_ml_prog_state ())>>
   reverse (Cases_on `STD_streams fs`) >- (fs [TextIOProofTheory.STDIO_def] \\ xpull) >>
   xlet_autop>>
   Cases_on`res`>>fs[SUM_TYPE_def]
-  >- (
-    xmatch>>
-    xapp_spec output_stderr_spec \\ xsimpl>>
-    asm_exists_tac>>xsimpl>>
-    qexists_tac`emp`>>xsimpl>>
-    qexists_tac`fs`>>xsimpl>>
-    rw[]>>
-    qexists_tac`x`>>xsimpl>>rw[]>>
-    fs[STD_streams_add_stderr, STD_streams_stdout,add_stdo_nil]>>
-    xsimpl)
   >- (
     xmatch>>
     xapp_spec output_stderr_spec \\ xsimpl>>
@@ -292,55 +206,51 @@ Proof
     asm_exists_tac>>simp[]>>
     qexists_tac`emp`>>qexists_tac`fs`>>xsimpl>>
     rw[]>>
-    qexists_tac`print_mccis_bound x`>>simp[]>>
+    qexists_tac`print_clique_bound x`>>simp[]>>
     qexists_tac`strlit ""`>>
     rw[]>>simp[STD_streams_stderr,add_stdo_nil]>>
     xsimpl>>
-    (drule_at Any) full_encode_mccis_sem_concl>>
+    (drule_at Any) full_encode_sem_concl>>
     fs[]>>
     Cases_on`x`>> disch_then (drule_at Any)>>
-    disch_then(qspec_then`gt'` mp_tac)>>
-    impl_tac>-
-      fs[get_graph_lad_def,AllCaseEqs()]>>
+    impl_tac>- (
+      fs[get_graph_dimacs_def,AllCaseEqs()]>>
+      metis_tac[parse_dimacs_good_graph])>>
     rw[]>>
     qexists_tac`(q,r)`>>
-    simp[mccis_sem_def]>>
+    simp[clique_sem_def]>>
     metis_tac[])
 QED
 
-Definition check_unsat_2_sem_def:
-  check_unsat_2_sem fs f1 f2 out ⇔
-  case get_graph_lad fs f1 of
+Definition check_unsat_1_sem_def:
+  check_unsat_1_sem fs f1 out ⇔
+  case get_graph_dimacs fs f1 of
     NONE => out = strlit ""
-  | SOME gpp =>
-  case get_graph_lad fs f2 of
-    NONE => out = strlit ""
-  | SOME gtt =>
-    out = concat (print_pbf (full_encode_mccis gpp gtt))
+  | SOME g =>
+    out = concat (print_pbf (full_encode g))
 End
 
-val check_unsat_2 = (append_prog o process_topdecs) `
-  fun check_unsat_2 f1 f2 =
-  case parse_and_enc f1 f2 of
+val check_unsat_1 = (append_prog o process_topdecs) `
+  fun check_unsat_1 f1 =
+  case parse_and_enc f1 of
     Inl err => TextIO.output TextIO.stdErr err
   | Inr (n,objf) =>
     TextIO.print_list (print_pbf objf)`
 
-Theorem check_unsat_2_spec:
+Theorem check_unsat_1_spec:
   STRING_TYPE f1 f1v ∧ validArg f1 ∧
-  STRING_TYPE f2 f2v ∧ validArg f2 ∧
   hasFreeFD fs
   ⇒
-  app (p:'ffi ffi_proj) ^(fetch_v"check_unsat_2"(get_ml_prog_state()))
-    [f1v;f2v]
+  app (p:'ffi ffi_proj) ^(fetch_v"check_unsat_1"(get_ml_prog_state()))
+    [f1v]
     (STDIO fs)
     (POSTv uv. &UNIT_TYPE () uv *
     SEP_EXISTS out err.
       STDIO (add_stdout (add_stderr fs err) out) *
-      &(check_unsat_2_sem fs f1 f2 out))
+      &(check_unsat_1_sem fs f1 out))
 Proof
-  rw[check_unsat_2_sem_def]>>
-  xcf "check_unsat_2" (get_ml_prog_state ())>>
+  rw[check_unsat_1_sem_def]>>
+  xcf "check_unsat_1" (get_ml_prog_state ())>>
   reverse (Cases_on `STD_streams fs`) >- (fs [TextIOProofTheory.STDIO_def] \\ xpull) >>
   xlet_autop>>
   Cases_on`res`>>fs[SUM_TYPE_def]
@@ -349,15 +259,6 @@ Proof
     xapp_spec output_stderr_spec \\ xsimpl>>
     asm_exists_tac>>xsimpl>>
     qexists_tac`emp`>>qexists_tac`fs`>>xsimpl>>
-    fs[STD_streams_add_stderr, STD_streams_stdout,add_stdo_nil]>>
-    rw[]>>
-    qexists_tac`x`>>xsimpl)
-  >- (
-    xmatch>>
-    xapp_spec output_stderr_spec \\ xsimpl>>
-    asm_exists_tac>>xsimpl>>
-    qexists_tac`emp`>>qexists_tac`fs`>>xsimpl>>
-    every_case_tac>>xsimpl>>
     fs[STD_streams_add_stderr, STD_streams_stdout,add_stdo_nil]>>
     rw[]>>
     qexists_tac`x`>>xsimpl)>>
@@ -374,7 +275,7 @@ Proof
 QED
 
 Definition usage_string_def:
-  usage_string = strlit "Usage: cake_pb_mccis <LAD file (pattern)> <LAD file (target)> <optional: PB proof file>\n"
+  usage_string = strlit "Usage: cake_pb_clique <DIMACS file> <optional: PB proof file>\n"
 End
 
 val r = translate usage_string_def;
@@ -382,16 +283,16 @@ val r = translate usage_string_def;
 val main = (append_prog o process_topdecs) `
   fun main u =
   case CommandLine.arguments () of
-    [f1,f2] => check_unsat_2 f1 f2
-  | [f1,f2,f3] => check_unsat_3 f1 f2 f3
+    [f1] => check_unsat_1 f1
+  | [f1,f2] => check_unsat_2 f1 f2
   | _ => TextIO.output TextIO.stdErr usage_string`
 
 Definition main_sem_def:
   main_sem fs cl out =
-  if LENGTH cl = 3 then
-    check_unsat_2_sem fs (EL 1 cl) (EL 2 cl) out
-  else if LENGTH cl = 4 then
-    check_unsat_3_sem fs (EL 1 cl) (EL 2 cl) out
+  if LENGTH cl = 2 then
+    check_unsat_1_sem fs (EL 1 cl) out
+  else if LENGTH cl = 3 then
+    check_unsat_2_sem fs (EL 1 cl) out
   else out = strlit ""
 End
 
@@ -435,23 +336,11 @@ Proof
   Cases_on`t'`>>fs[LIST_TYPE_def]
   >- (
     xmatch>>
-    xapp_spec output_stderr_spec \\ xsimpl>>
-    rename1`COMMANDLINE cl`>>
-    qexists_tac`COMMANDLINE cl`>>xsimpl>>
-    qexists_tac `usage_string` >>
-    simp [theorem "usage_string_v_thm"] >>
-    qexists_tac`fs`>>xsimpl>>
-    rw[]>>
-    fs[STD_streams_add_stderr, STD_streams_stdout,add_stdo_nil]>>
-    metis_tac[STDIO_refl])>>
-  Cases_on`t`>>fs[LIST_TYPE_def]
-  >- (
-    xmatch>>
     xapp>>rw[]>>
     rpt(first_x_assum (irule_at Any)>>xsimpl)>>
     fs[wfcl_def]>>
     rw[]>>metis_tac[STDIO_refl])>>
-  Cases_on`t'`>>fs[LIST_TYPE_def]
+  Cases_on`t`>>fs[LIST_TYPE_def]
   >- (
     xmatch>>
     xapp>>rw[]>>
