examples/pseudo_bool/graph_encoding/graph_basicScript.sml
@@ -5,22 +5,26 @@ open preamble mlintTheory;
 
 val _ = new_theory "graph_basic";
 
-(* Graph: (V : num , E : (num list) num_map)
+(* Graph: (V : num , E : (num_set) num_map)
   V number of vertices
   E edge list representation *)
 
-Type edges = ``:(num list) num_map``;
+Type edges = ``:num_set num_map``;
 Type graph = ``:num # edges``;
 
 (* Edge from a -> b in edge list representation e *)
 Definition is_edge_def:
   is_edge (e:edges) (a:num) (b:num) ⇔
-  case lookup a e of SOME ns => MEM b ns | _ => F
+  case lookup a e of
+    SOME ns => lookup b ns = SOME ()
+  | _ => F
 End
 
 Theorem is_edge_thm:
   is_edge e a b ⇔
-  ∃ns. lookup a e = SOME ns ∧ MEM b ns
+  ∃ns.
+    lookup a e = SOME ns ∧
+    lookup b ns = SOME ()
 Proof
   rw[is_edge_def]>>every_case_tac>>fs[]
 QED
@@ -28,28 +32,54 @@ QED
 (* A "good" graph is undirected and only mentions edges < v *)
 Definition good_graph_def:
   good_graph ((v,e):graph) ⇔
-  ∀a ns.
-    sptree$lookup a e = SOME ns ⇒ a < v ∧
-    ∀b. is_edge e a b ⇒ is_edge e b a
+  domain e ⊆ count v ∧
+  ∀a b. is_edge e a b ⇒ is_edge e b a
 End
 
+Theorem good_graph_eq:
+  good_graph (v,e) ⇔
+  ∀a ns.
+    (sptree$lookup a e = SOME ns ⇒
+      a < v ∧
+      (∀b. is_edge e a b ⇒ is_edge e b a))
+Proof
+  rw[good_graph_def,EQ_IMP_THM,SUBSET_DEF,domain_lookup]>>
+  fs[is_edge_thm]
+QED
+
+Definition neighbours_sp_def:
+  neighbours_sp e v =
+  case lookup v e of
+    NONE => LN
+  | SOME ns => ns
+End
+
+Theorem lookup_neighbours_sp:
+  lookup b (neighbours_sp e a) = SOME () ⇔
+  is_edge e a b
+Proof
+  rw[neighbours_sp_def,is_edge_thm]>>
+  every_case_tac>>
+  fs[]
+QED
+
+(* Neighbors as a sorted list *)
 Definition neighbours_def:
   neighbours (e:edges) (v:num) =
-  case lookup v e of NONE => [] | SOME ns => ns
+  MAP FST (toSortedAList (neighbours_sp e v))
 End
 
 Theorem MEM_neighbours:
   MEM b (neighbours ep a) ⇔
   is_edge ep a b
 Proof
-  rw[neighbours_def,is_edge_thm]>>
-  every_case_tac>>fs[]
+  fs[MEM_toSortedAList,MEM_MAP,EXISTS_PROD,neighbours_def,lookup_neighbours_sp]
 QED
 
 Definition not_neighbours_def:
   not_neighbours (v,e) a =
-  let n = neighbours e a in
-  FILTER (λu. ¬ MEM u n) (COUNT_LIST v)
+  let n = neighbours_sp e a in
+  FILTER (λu. lookup u n ≠ SOME ()) (COUNT_LIST v)
 End
 
 Theorem MEM_not_neighbours:
@@ -57,12 +87,80 @@ Theorem MEM_not_neighbours:
   b < vp ∧
   ¬is_edge ep a b
 Proof
-  rw[not_neighbours_def,MEM_FILTER,is_edge_thm,neighbours_def]>>
-  every_case_tac>>fs[MEM_COUNT_LIST]>>
+  rw[not_neighbours_def,MEM_FILTER,lookup_neighbours_sp,MEM_COUNT_LIST]>>
   metis_tac[]
 QED
 
-(* Parser for LAD *)
+Definition insert_dir_edge_def:
+  insert_dir_edge e u v =
+  let ns = neighbours_sp e u in
+  let nsv = insert v () ns in
+  insert u nsv e
+End
+
+Definition insert_edge_def:
+  insert_edge e u v =
+  insert_dir_edge
+    (insert_dir_edge e u v) v u
+End
+
+Theorem is_edge_insert_dir_edge:
+  is_edge (insert_dir_edge e u v) x y ⇔
+  is_edge e x y ∨
+  x = u ∧ y = v
+Proof
+  rw[insert_dir_edge_def,is_edge_thm]>>
+  every_case_tac>>
+  rw[lookup_insert]>>
+  rw[]>>
+  fs[lookup_neighbours_sp,is_edge_thm]
+QED
+
+Theorem is_edge_insert_edge:
+  is_edge (insert_edge e u v) x y ⇔
+  is_edge e x y ∨
+  x = u ∧ y = v ∨
+  x = v ∧ y = u
+Proof
+  rw[is_edge_insert_dir_edge,insert_edge_def]>>
+  metis_tac[]
+QED
+
+Theorem domain_insert_dir_edge:
+  domain (insert_dir_edge e x y) = domain e ∪ {x}
+Proof
+  rw[insert_dir_edge_def]>>
+  every_case_tac>>rw[]>>
+  metis_tac[INSERT_SING_UNION,UNION_COMM]
+QED
+
+Theorem domain_insert_edge:
+  domain (insert_edge e x y) = domain e ∪ {x;y}
+Proof
+  rw[insert_edge_def,domain_insert_dir_edge]>>
+  simp[EXTENSION]>>
+  metis_tac[]
+QED
+
+Theorem good_graph_insert_edge:
+  good_graph (v,e) ∧
+  x < v ∧ y < v ⇒
+  good_graph (v,insert_edge e x y)
+Proof
+  rw[good_graph_def]
+  >-
+    simp[domain_insert_edge]
+  >-
+    fs[is_edge_insert_edge]
+QED
+
+(* Parsers *)
+
+(* Everything recognized as a "blank" *)
+Definition blanks_def:
+  blanks (c:char) ⇔ c = #" " ∨ c = #"\n" ∨ c = #"\t" ∨ c = #"\r"
+End
+
 Definition tokenize_num_def:
   tokenize_num (s:mlstring) =
   case mlint$fromNatString s of
@@ -70,45 +168,132 @@ Definition tokenize_num_def:
   | SOME i => INR i
 End
 
-(* TODO: copied from lpr_parsing *)
-(* Everything recognized as a "blank" *)
-Definition blanks_def:
-  blanks (c:char) ⇔ c = #" " ∨ c = #"\n" ∨ c = #"\t" ∨ c = #"\r"
-End
-
 Definition toks_num_def:
   toks_num s = MAP tokenize_num (tokens blanks s)
 End
 
-Definition parse_num_list_def:
-  (parse_num_list v [] acc = SOME (REVERSE acc)) ∧
-  (parse_num_list v (x::xs) acc =
+(* Parser for LAD
+  Assumptions:
+  - The file must provide both (undirected) edges
+*)
+Definition parse_lad_num_list_def:
+  (parse_lad_num_list v [] acc = SOME (REVERSE acc)) ∧
+  (parse_lad_num_list v (x::xs) acc =
     case x of
-      INR (n:num) => parse_num_list v xs (n::acc)
+      INR (n:num) => parse_lad_num_list v xs (n::acc)
     | INL _ => NONE)
 End
 
-(* A parser for LAD format *)
-Definition parse_edges_def:
-  (parse_edges v i [] acc = SOME acc) ∧
-  (parse_edges v i (l::ls) acc =
-    case parse_num_list v l [] of
+Definition parse_lad_edges_def:
+  (parse_lad_edges v i [] acc = SOME acc) ∧
+  (parse_lad_edges v i (l::ls) acc =
+    case parse_lad_num_list v l [] of
       SOME (d::xs) =>
-        if LENGTH xs = d then parse_edges v (i+1) ls (insert i xs acc) else NONE
+        if LENGTH xs = d then
+          parse_lad_edges v (i+1) ls (insert i (list_to_num_set xs) acc)
+        else NONE
     | _ => NONE)
 End
 
-Definition check_good_edges_inner_def:
-  check_good_edges_inner u v es =
-  case lookup u es of NONE => F
-      | SOME edges => MEM v edges
+Definition parse_lad_toks_def:
+  parse_lad_toks ls =
+  case ls of
+    [INR h]::rest =>
+      (case parse_lad_edges h 0 rest LN of NONE => NONE
+      | SOME e => SOME (h,e))
+  | _ => NONE
 End
+
+Definition parse_lad_def:
+  parse_lad lines = parse_lad_toks (MAP toks_num lines)
+End
+
+(* Parser for DIMACS
+  Assumptions:
+  - The file may provide edges in only one direction
+    (they are automatically made into undirected edges)
+*)
+Definition nocomment_line_def:
+  (nocomment_line (INL c::cs) = (c ≠ strlit "c")) ∧
+  (nocomment_line _ = T)
+End
+
+Definition parse_dimacs_header_def:
+  (parse_dimacs_header [INL p; INL lab; INR v; INR e] =
+    if p = strlit"p" ∧
+       (lab = strlit "col" ∨ lab = strlit"edge")
+    then SOME (v:num,e:num)
+    else NONE) ∧
+  parse_dimacs_header _ = NONE
+End
+
+(* To keep the internal representation with LAD,
+  we use 0-indexing *)
+Definition parse_dimacs_edge_def:
+  parse_dimacs_edge v ls =
+    case ls of [INL e; INR (x:num); INR (y:num)] =>
+      if e = strlit"e" ∧ x > 0 ∧ x ≤ v ∧ y > 0 ∧ y ≤ v
+      then
+        SOME (x - 1, y - 1)
+      else NONE
+    | _ => NONE
+End
+
+Definition parse_dimacs_edges_def:
+  (parse_dimacs_edges v [] acc = SOME acc) ∧
+  (parse_dimacs_edges v (l::ls) acc =
+    case parse_dimacs_edge v l of
+      SOME (x,y) =>
+        parse_dimacs_edges v ls (insert_edge acc x y)
+    | _ => NONE)
+End
+
+Definition parse_dimacs_toks_def:
+  parse_dimacs_toks lines =
+  case FILTER nocomment_line lines of
+    [] => NONE
+  | (h::xs) =>
+    (case parse_dimacs_header h of NONE => NONE
+    | SOME (v,e) =>
+      (case parse_dimacs_edges v xs LN of
+        NONE => NONE
+      | SOME es => SOME (v,es)))
+End
+
+Definition parse_dimacs_def:
+  parse_dimacs lines = parse_dimacs_toks (MAP toks_num lines)
+End
+
+Theorem parse_dimacs_edges_good_graph:
+  ∀lines acc es.
+  good_graph (v,acc) ∧
+  parse_dimacs_edges v lines acc = SOME es ⇒
+  good_graph (v,es)
+Proof
+  Induct>>rw[parse_dimacs_edges_def]>>
+  gvs[AllCaseEqs()]>>
+  first_x_assum match_mp_tac>>
+  first_x_assum (irule_at Any)>>
+  match_mp_tac good_graph_insert_edge>>
+  fs[parse_dimacs_edge_def,AllCaseEqs()]
+QED
+
+Theorem parse_dimacs_good_graph:
+  parse_dimacs lines = SOME g ⇒
+  good_graph g
+Proof
+  rw[parse_dimacs_def,parse_dimacs_toks_def]>>
+  gvs[AllCaseEqs()]>>
+  match_mp_tac parse_dimacs_edges_good_graph>>
+  first_x_assum (irule_at Any)>>
+  fs[good_graph_def,is_edge_def]
+QED
 
 (* Undirectedness and u < bound *)
 Definition check_good_edges_def:
   check_good_edges bound v ls es =
-    EVERY (λu.
-      check_good_edges_inner u v es) ls
+    EVERY (λ(u,_).
+      is_edge es u v) (toAList ls)
 End
 
 Definition check_good_graph_def:
@@ -121,12 +306,16 @@ Theorem check_good_graph:
   check_good_graph (v,e) ⇒
   good_graph (v,e)
 Proof
-  rw[good_graph_def,check_good_graph_def,is_edge_def]>>
+  rw[good_graph_eq,check_good_graph_def,is_edge_def]>>
   fs[GSYM MEM_toAList,EVERY_MEM]>>
+  fs[MEM_toAList,FORALL_PROD]>>
   first_x_assum drule>>
-  fs[check_good_edges_def,check_good_edges_inner_def]>>
+  fs[check_good_edges_def]>>
   rw[]>>
-  fs[EVERY_MEM]
+  fs[EVERY_MEM,MEM_toAList,FORALL_PROD]>>
+  first_x_assum drule>>simp[is_edge_thm]>>
+  rw[]>>
+  simp[]
 QED
 
 Theorem check_good_graph_iff:
@@ -135,28 +324,16 @@ Theorem check_good_graph_iff:
 Proof
   Cases_on`g`>>
   simp[EQ_IMP_THM,check_good_graph]>>
-  rw[good_graph_def,check_good_graph_def,is_edge_def]>>
-  fs[GSYM MEM_toAList,EVERY_MEM]>>
-  simp[FORALL_PROD]>>
-  rw[]>>
+  rw[good_graph_eq,check_good_graph_def,is_edge_def]>>
+  fs[GSYM MEM_toAList,EVERY_MEM,FORALL_PROD]>>
+  fs[MEM_toAList]>>rw[]>>
   first_x_assum drule>>
-  fs[check_good_edges_def,check_good_edges_inner_def]>>
+  fs[check_good_edges_def]>>
   rw[]>>
-  fs[EVERY_MEM]
+  fs[EVERY_MEM,FORALL_PROD,MEM_toAList]>>rw[]>>
+  first_x_assum drule>>fs[is_edge_thm]>>
+  every_case_tac>>fs[]
 QED
-
-Definition parse_lad_toks_def:
-  parse_lad_toks ls =
-  case ls of
-    [INR h]::rest =>
-      (case parse_edges h 0 rest LN of NONE => NONE
-      | SOME e => SOME (h,e))
-  | _ => NONE
-End
-
-Definition parse_lad_def:
-  parse_lad lines = parse_lad_toks (MAP toks_num lines)
-End
 
 val ladraw = ``[
   strlit"5";
@@ -178,5 +355,21 @@ val ladraw = ``[
 ]``;
 
 val pattern = rconc (EVAL``check_good_graph (THE (parse_lad ^ladraw))``)
+
+(* DIMACS *)
+
+val dimraw = ``[
+strlit"c edge density";
+strlit"c min degree";
+strlit"p col 125 6963";
+strlit"e 2 1";
+strlit"e 3 1";
+strlit"e 4 1";
+strlit"e 5 1";
+strlit"e 5 2";
+strlit"e 5 3";
+]``;
+
+val pattern = rconc (EVAL``(THE (parse_dimacs ^dimraw))``)
 
 val _ = export_theory();
